% --------------------------------------------------------------
% This is all preamble stuff that you don't have to worry about.
% Head down to where it says "Start here"
% --------------------------------------------------------------
 
\documentclass[12pt]{article}
 
\usepackage[margin=1in]{geometry} 
\usepackage{amsmath,amsthm,amssymb}
 
\newcommand{\N}{\mathbb{N}}
\newcommand{\Z}{\mathbb{Z}}
 
\newenvironment{theorem}[2][Theorem]{\begin{trivlist}
\item[\hskip \labelsep {\bfseries #1}\hskip \labelsep {\bfseries #2.}]}{\end{trivlist}}
\newenvironment{lemma}[2][Lemma]{\begin{trivlist}
\item[\hskip \labelsep {\bfseries #1}\hskip \labelsep {\bfseries #2.}]}{\end{trivlist}}
\newenvironment{exercise}[2][Exercise]{\begin{trivlist}
\item[\hskip \labelsep {\bfseries #1}\hskip \labelsep {\bfseries #2.}]}{\end{trivlist}}
\newenvironment{problem}[2][Problem]{\begin{trivlist}
\item[\hskip \labelsep {\bfseries #1}\hskip \labelsep {\bfseries #2.}]}{\end{trivlist}}
\newenvironment{question}[2][Question]{\begin{trivlist}
\item[\hskip \labelsep {\bfseries #1}\hskip \labelsep {\bfseries #2.}]}{\end{trivlist}}
\newenvironment{corollary}[2][Corollary]{\begin{trivlist}
\item[\hskip \labelsep {\bfseries #1}\hskip \labelsep {\bfseries #2.}]}{\end{trivlist}}
 
\begin{document}
 
% --------------------------------------------------------------
%                         Start here
% --------------------------------------------------------------
 
\title{Assignment 7}%replace X with the appropriate number
\author{Md Ali\\ %replace with your name
Combinatorics 4350} %if necessary, replace with your course title
 
\maketitle
 
\begin{problem}{1} %You can use theorem, exercise, problem, or question here.  Modify x.yz to be whatever number you are proving
Let $\{ a_n \}_{n \geq 0}$ be a real sequence with generating function $F(x)$. $(i.e. F(x) \sum_{n=0}^{\infty} a_n)$. Find an expression for $a_n$ for every non-negative integer $n$, if \\ \\ 
\centerline{$F(x) = \dfrac{18+2x^3}{(1-x)^3}$} \\ \\

\end{problem}

\begin{proof}
Switching up our generating function we get \\ \\
\centerline{ $\dfrac{18+2x^3}{(1-x)^3} =  2\dfrac{9+x^3}{(1-x)^3} =  2\dfrac{9+x^3}{(1-x)^2(1-x^2)}$} \\ \\
\centerline{ $2\dfrac{9+x^3}{(1-x)^2(1-x^2)} = 2(9+x^3)(1-x^2)^{-1}(1-x)^{-2}$} \\ \\
Using the table for generating function \\ \\
\centerline{$F(x) = 2(9+x^3)(1+x^2+x^4+...)(1+2x+3x^2+...)$} \\ \\
\centerline{$F(x) = 2(9+x^3)(1+2x+3x^2+4x^3...+x^2+2x^3+3x^4+4x^5+...)$} \\ \\
\centerline{$F(x) = 2[9+18x+36x^2 +54x^3+...]$} \\ \\
\centerline{$F(x) = 18+36x+72x^2+108x^3+...$} \\ \\
So we get that \\ \\
\centerline{$a_n = a_{n-1}+a_{n-2}$ with $a_0=18,a_1 = 36, a_2 = 72$} \\ \\

\end{proof}

\begin{problem}{2}
Determine the coefficients of $x^{30}$ and of $x^{37}$ in the formal power series for the ordinary generating function
$$F(x)={{3x^2}\over {1-2x^7}}+{2\over {(1-x)^5}}+{{20+5x}\over {1-x^2}}.$$
\end{problem}

\begin{proof}
We want to find $x^{30}$ and of $x^{37}$ \\ \\
\centerline{$F(x) = 3(x^2)(1-2x^7)^{-1}+2(1-x)^{-5}+(20+5x)(1-x^2)^{-1}$} \\ \\
Used Mathematica to find each coefficient \\ \\
\centerline{$x^{30} = 2357065$, $x^{37}=58331641$} \\ \\
\end{proof}

\begin{problem}{3}
Let $\{a_n\}_{n\geq 0}$ be a real sequence with ordinary generating function $F(x)$, i.e. $F(x)=\sum_{n=0}^{\infty}a_nx^n$. Let $k$ be an arbitrary positive integer.
Let $\{b_n\}_{n\geq 0}$ be the sequence defined by $b_n={{n+k}\choose n}k!a_{n+k}$, for any non-negative integer $n$, and let $G(x)$ be the ordinary generating function for the sequence $\{b_n\}_{n\geq 0}$. Express $G(x)$ in terms of $F(x)$, $\{a_n\}_{n\geq 0}$ and the integer $k$.\\
\end{problem}

\begin{proof}
Let's look at first \\ \\
\centerline{${n+k \choose n} = \dfrac{(n+k)!}{n!(n+k-n)!} \rightarrow  \dfrac{(n+k)!}{n!(n+k-n)!}  \cdot k! \cdot a_{n+k} = \dfrac{(n+k)!}{n!}\cdot a_{n+k}$} \\ \\
\centerline{ $\sum_{n=0}^{\infty} \dfrac{(n+k)!}{n!}\cdot a_{n+k}x^{n+k}$} \\ \\
\centerline{$\dfrac{(n+k)!}{n!} = k! - n!$} \\ \\
\centerline{$\sum_{n=0}^{\infty} (k! - n!)\cdot a_{n+k}x^{n+k}$} \\ \\
\centerline{$\sum_{n=0}^{\infty} k!\cdot a_{n+k}x^{n+k} - n! \cdot a_{n+k}x^{n+k}$} \\ \\
\centerline{$k!\sum_{n=0}^{\infty} a_{n+k}x^{n+k} - n! \cdot a_{n+k}x^{n+k}$} \\ \\
Not sure what to do from here.


\end{proof}
 
\begin{problem}{4}
Let $\{a_n\}_{n\geq 0}$ be a real sequence with ordinary generating function $F(x)$, i.e. $F(x)=\sum_{n=0}^{\infty}a_nx^n$. Let $s$ and $t$ be two positive integers. Let $\{b_n\}_{n\geq 0}$ be the sequence defined by 
$$b(n)=\left\{
	\begin{array}{ll}
	0, & \mbox {if } 0\leq n\leq 3 \\
	ta_{n}-1,  & \mbox {if } n\geq 4 \mbox{ and } n \mbox{ is even} \\
	sa_{n}+1, & \mbox {if } n\geq 5 \mbox{ and } n \mbox{ is odd}
	\end{array}
	\right.$$
and let $G(x)$ be the ordinary generating function for the sequence $\{b_n\}_{n\geq 0}$. Express $G(x)$ in terms of $F(x)$, $\{a_n\}_{n\geq 0}$ and the integers $s$ and $t$.\\
\end{problem}

\begin{proof} 
I had no idea where to start. At least I'm trying I suppose.
\end{proof}



% --------------------------------------------------------------
%     You don't have to mess with anything below this line.
\end{document}